src/ITreeSpec/ITreeSpecDefinition.v
@@ -53,13 +53,6 @@ Definition itree_spec (E : Type -> Type) (R : Type) :=
 
 Notation itree_spec' E R := (itree' (SpecEvent E) R).
 
-#[global] Instance itree_spec_MonadEq1 {E} : Eq1 (itree_spec E).
-red.
-unfold itree_spec.
-intros A.
-apply eq1.
-Defined.
-
 #[global] Instance Monad_itree_spec {E} : Monad (itree_spec E).
 unfold itree_spec.
 constructor.
